% !TEX root = ../calibreport.tex
%============================================

Let us consider the equation:
$$
 Y_{t}=g_{t} \star X_{t}
$$
where $g_{t}$ is the $M$-ary impulse response of the single input multiple output (SIMO) linear filter and $X_{t}$ is a scalar WSS process, with zero mean and spectral matrix (of size 1) $\gamma_{x}(f)$. It is easy to show that the spectral matrix of $Y_{t}$ writes
$$
 \Sigma_{y}(f)=\gamma_{x}(f)G(f)G^{H}(f)
$$
where $G(f)$ is the discrete time Fourier transform of $g_{t}$.
We notice that $\Sigma_{y}(f)$ is a matrix of rank 1. A particular case is a pure delay propagation filter as for example in the planar propagation where the vector entry of $G(f)$ writes:
$$
 G_{m}(f)=e^{-2j\pi f r_{m}^{T}\theta}
$$
where $r_{m}$ is the 3D location of the sensor $m$ and $\theta$ the wave number of the planar wave. It follows that the coherence matrix of the $M$-ary observation has the following entry expression
\begin{eqnarray}
 \label{eq:delaymatrixpuredelay}
 C_{y,m\ell}(f)&=&e^{-2j\pi f (r_{m}-r_{\ell})^{T}\theta}
 \\ \nonumber
 &=&\int_{\mathds{R}^{3}} e^{-2j\pi f (r_{m}-r_{\ell})^{T}u}\delta_{\theta}(u)du
\end{eqnarray}
where $du$ is the infinitesimal Lebesgue measure in $\mathds{R}^{3}$ and $\delta_{\theta}$ the Dirac's distribution located in $\theta$. The expression \eqref{eq:delaymatrixpuredelay} can be seen as an expectation of $e^{-2j\pi f (r_{m}-r_{\ell})^{T}\theta}$ assuming that $\theta$ is deterministic.

%===================================================================
\subsubsection{Coherence model}

In a pioneer work Mack and Flinn \cite{mack_flinn:1971} propose to model the loss of coherence by considering that the azimuth, the elevation and velocity are uncertain. More specifically, authors in \cite{nouvellet:2012}  assume that the 3D vector $\mu=(a,e,c)$ where $a$ denotes the azimuth, $e$ the elevation and $c$ the sound velocity writes:
\begin{equation}
 \label{eq:randomnesswn}
 \mu=\mu_{0}+\nu
\end{equation} 
where $\mu_{0}=(a_{0},e_{0},c_{0})$ is a deterministic value and $\nu$ a zero-mean Gaussian random vector of dimension 3, whose covariance is denoted $\Sigma_{\mu}$.  We know that $\mu$ is related to the slowness vector $k$ by the one-to-one mapping 
\begin{eqnarray*}
 \label{eq:tehtaxyz}
 {\footnotesize
 \begin{array}{rcl}
 f:\,
  \mu= 
 \left\{
 \begin{array}{ll}
 a=\arg(k_{2}+jk_{1})&a\in(0,2\pi)
 \\
 e=\arg\sin(ck_{3})&e\in(-\pi/2,\pi/2)
 \\
 v=(k_{1}^{2}+k_{2}^{2}+k_{3}^{2})^{1/2}&v\in\mathds{R}^{+}
 \end{array}\right.
 &
 \Longleftrightarrow\vspace{6pt}
 \\ 
 &&\hspace{-5.5cm}
 \,k=\left\{
 \begin{array}{ll}
 k_{1}=-v^{-1}\sin(a)\cos(e)
 \\
 k_{2}=v^{-1}\cos(a)\cos(e)&\in\mathds{R}^{3}
 \\
 k_{3}=v^{-1}\sin(e) 
 \end{array}\right.
 \end{array}}
\end{eqnarray*}
Using a first order Taylor's expansion, it follows that $k \approx f(\mu_{0})+J(\mu_{0})(\mu-\mu_{0})$ where the Jacobian writes
\begin{eqnarray*}
 J(\mu_{0}) 
&=&
v_{0}^{-1} \times \tilde J(\mu_0)
\\
\mathrm{with}&&
\tilde J(\mu_0) = 
\begin{bmatrix}
 -\cos(a_{0})\cos(e_{0})&
 \sin(a_{0})\sin(e_{0})&
 v_{0}^{-1}\sin(a_{0})\cos(e_{0})
 \\
 -\sin(a_{0})\cos(e_{0})&
 -\cos(a_{0})\sin(e_{0})&
 -v_{0}^{-1}\cos(a_{0})\cos(e_{0})
 \\
 0& 
 \cos(e_{0})&
 -v_{0}^{-1}\sin(e_{0})
 \end{bmatrix}
\end{eqnarray*}
Therefore from \eqref{eq:randomnesswn} we derive $k\approx k_{0}+\varepsilon$ where $\varepsilon=J(\mu_{0})\,\nu$ appears as a zero-mean Gaussian random vector whose the covariance is:
\begin{eqnarray}
 \label{eq:aec2theta}
\Sigma_{k} \approx v_{0}^{-2} 
\underbrace{\tilde J(\mu_{0}) \Sigma_{\mu} \tilde J^{T}(\mu_{0})}_{\tilde \Sigma_{k}}
\end{eqnarray}
Hence the coherence matrix entry of the model with random wavefront writes:
\begin{eqnarray*}
   C_{m,\ell}(f)&=&e^{-2j\pi f(r_{m}-r_{\ell})^{T}k_{0}}
   \Phi_{\epsilon}(2\pi f(r_{m}-r_{\ell}))
\end{eqnarray*}
where $\Phi_{\epsilon}:u\in\mathds{R}^{3}\mapsto\esp{e^{ju^{T}\varepsilon}}\in\mathds{C}$ is the characteristic function of $\varepsilon$. 
Since $\varepsilon$ is Gaussian distributed with zero-mean and covariance matrix $\Sigma_{k}$, hence we have
\begin{eqnarray}
\label{eq:Cfr1r2Gaussian}
C_{m,\ell}(f)=
\underbrace{e^{-2j\pi f(r_{m}-r_{\ell})^{T}k_{0}}}_{\text{pure delay}}
 \underbrace{e^{-2\pi^{2}(f/v_0)^{2}(r_{m}-r_{\ell})^{T}
                 \tilde \Sigma_{k}(r_{m}-r_{\ell})}}_{\text{LOC}}
 \end{eqnarray}

We let  $\zeta=v_0/f$ that can be interpreted as a ``wavelength''. Using the MSC definition \eqref{eq:def-coherence-function}  we derive the following expression:
\begin{eqnarray}
\label{eq:MSCwind}
\MSC_{km}(f)=
e^{-\frac{4\pi^{2}}{\zeta^{2}}(r_{m}-r_{\ell})^{T}
                 \tilde \Sigma_{k}(r_{m}-r_{\ell})}
 \end{eqnarray}
It follows that
\begin{itemize}
\item
 when $\zeta$ is large w.r.t. the sensor  inter-distances, the matrix $C\approx I$, hence the components of $x(t)$ appear as non spatially coherent,


\item
when $\zeta$ is small w.r.t.  the sensor  inter-distances, the matrix $C\approx \mathds{1} \mathds{1}^{T}$ which is a projector, hence the components of $x(t)$ appear as spatially coherent.
 

\end{itemize}
